Call Auctions/MM.v
@@ -12,25 +12,32 @@ FOA (Match (Decr_Bid.sort B) (Decr_Ask.sort A)) A.
 Theorem MM_Is_Matching (B:list order)(A:list order):
 admissible B A -> Matching (MM B A) B A.
 Proof. unfold MM. intros. apply FOA_correct. split. auto. eapply Maching_permutation_full with (A1:=(Decr_Ask.sort A))
-(B1:=(Decr_Bid.sort B)). admit. admit. exact. 
- apply Match_Matching. admit. admit. 
- Admitted.
+(B1:=(Decr_Bid.sort B)). apply perm_sym. apply Permulation_perm. apply Decr_Bid.Permuted_sort. 
+apply perm_sym. apply Permulation_perm. apply Decr_Ask.Permuted_sort. exact. 
+ apply Match_Matching. 
+apply perm_nodup with (l:=(ids A)). apply ids_perm. apply Permulation_perm. apply Decr_Ask.Permuted_sort. apply H. 
+apply perm_nodup with (l:=(ids B)). apply ids_perm. apply Permulation_perm. apply Decr_Bid.Permuted_sort. apply H.
+ Qed.
 
 Theorem MM_Is_fair (B:list order)(A:list order):
 admissible B A -> Is_fair (MM B A) B A.
 Proof. unfold MM. unfold Is_fair.
 intros. split.
 { eapply FOA_correct. split. exact H. eapply Maching_permutation_full with (A1:=(Decr_Ask.sort A))
-(B1:=(Decr_Bid.sort B)). admit. admit. exact. 
- apply Match_Matching. admit. admit. } 
-
+(B1:=(Decr_Bid.sort B)). apply perm_sym. apply Permulation_perm. apply Decr_Bid.Permuted_sort. 
+apply perm_sym. apply Permulation_perm. apply Decr_Ask.Permuted_sort. exact. 
+ apply Match_Matching. apply perm_nodup with (l:=(ids A)). apply ids_perm. apply Permulation_perm. apply Decr_Ask.Permuted_sort. apply H. apply perm_nodup with (l:=(ids B)). apply ids_perm. apply Permulation_perm. apply Decr_Bid.Permuted_sort. apply H. } 
 { eapply FOA_correct. split. exact H. eapply Maching_permutation_full with (A1:=(Decr_Ask.sort A))
-(B1:=(Decr_Bid.sort B)). admit. admit. exact. 
- apply Match_Matching. admit. admit. eapply Is_fair_bids_perm with (B1:=(Decr_Bid.sort B)) .
-exact. admit.
- apply Match_Fair_on_Bids. split. eapply admissible_perm. admit. admit. exact H. admit. } Admitted.
+(B1:=(Decr_Bid.sort B)). apply perm_sym. apply Permulation_perm. apply Decr_Bid.Permuted_sort.
+ apply perm_sym. apply Permulation_perm. apply Decr_Ask.Permuted_sort. exact. 
+ apply Match_Matching. apply perm_nodup with (l:=(ids A)). apply ids_perm. apply Permulation_perm. apply Decr_Ask.Permuted_sort. apply H. apply perm_nodup with (l:=(ids B)). apply ids_perm. apply Permulation_perm. apply Decr_Bid.Permuted_sort. apply H. eapply Is_fair_bids_perm with (B1:=(Decr_Bid.sort B)) .
+exact. apply perm_sym.  apply Permulation_perm. apply Decr_Bid.Permuted_sort.
+ apply Match_Fair_on_Bids. split. eapply admissible_perm. 
+apply Permulation_perm. apply Decr_Bid.Permuted_sort. 
+apply Permulation_perm. apply Decr_Ask.Permuted_sort.
+exact H. apply Decr_Bid.Sorted_sort. } Qed.
 
-
+(*
 (*Move this lemma into another file*)
 Lemma exists_ttq_top_bid 
 (B:list order)(A:list order)(M:list transaction)(b:order)
@@ -41,7 +48,7 @@ Sorted bcompetitive (b::B) ->
 (Qty_bid M' (id b) >= min (oquantity b) (Vol(M)))/\
 Vol(M) = Vol(M')).
 Proof. Admitted.
-(*
+
 Lemma MM_exists_opt_k (B A:list order)(b a: order)
 (NDA:NoDup (ids (a::A)))(NDB:NoDup (ids (b::B))):
 Sorted bcompetitive (b::B) -> 
@@ -190,374 +197,20 @@ Proof. intro Adm. intros.
 set(M0:= FOB M (b::B)). assert(Hf:= (FOB_correct M (b::B) (a::A))). 
 assert(admissible (b :: B) (a :: A) /\ Matching M (b :: B) (a :: A)). auto. apply Hf in H4 as H4a. destruct H4a.
 destruct H6. destruct H7. destruct ((min (oquantity b) (oquantity a)) - Qty (FOB M (b :: B)) (id b) (id a)) eqn:Hk.
-exists (FOB M (b :: B)). split. auto. split. (*Qty is never more than min a b, hence equal from H10.*) admit. auto.
+exists (FOB M (b :: B)). split. auto. split. 
+assert(HQb:= Qty_le_Qty_ask (FOB M (b :: B)) (id b) (id a)).
+assert(Qty_ask (FOB M (b :: B)) (id a) <= oquantity a). apply H5. auto.
+assert(HQa:= Qty_le_Qty_bid (FOB M (b :: B)) (id b) (id a)).
+assert(Qty_bid (FOB M (b :: B)) (id b) <= oquantity b). apply H5. auto. lia. auto.
 apply MM_exists_opt_k with (M:=(FOB M (b::B)))(A:=A)(B:=B)(k:=S n)(b:=b)(a:=a) in H5.
 destruct H5 as [M1 H5]. destruct H5. destruct H9. exists M1. split. auto.
-split. (*Qty is never more than min a b, hence equal from H10.*)
- admit. lia. 
+split. 
+assert(HQb:= Qty_le_Qty_ask (M1) (id b) (id a)).
+assert(Qty_ask (M1) (id a) <= oquantity a). apply H5. auto.
+assert(HQa:= Qty_le_Qty_bid (M1) (id b) (id a)).
+assert(Qty_bid (M1) (id b) <= oquantity b). apply H5. auto. lia. auto. lia. 
 all:auto. apply Adm. apply Adm. lia. apply (Is_FOB_ab_full_bid M B A b a).
-split. auto. split. auto. split. auto.  lia. Admitted. (*Use Qty_le_Qty_bid to clear admits *)
-
-
-(*
-Proof. intros. 
-       assert(exists M', (matching_in (b::B) (a::A) M')/\
-       (ttqb M' b >= min (bq b) (QM(M)))/\Is_IR M'/\QM(M)=QM(M')/\
-       forall m : fill_type, In m M' -> tq m > 0).
-       eapply exists_ttq_top_bid. all:auto. 
-       destruct H5 as [M0 H5].
-       destruct H5. destruct H6. destruct H7. 
-       destruct (Nat.min (bq b) (sq a) - ttq_ab M0 b a) eqn:Hk.
-       {
-         eapply MM_exists_opt_k with (k:=0)(A:=A)(a:=a)(B:=B)(b:=b) in H5.
-         destruct H5 as [OPT H5]. exists OPT. 
-         destruct H5. destruct H9.
-         split. apply H5. split. 
-         assert (Hmin:ttq_ab OPT b a <= Nat.min (bq b) (sq a)).
-         eapply matching_in_elim9 with (B:=(b::B))(A:=(a::A)).
-         apply H5. auto.
-         split. assert (Hmin:ttq_ab OPT b a <= Nat.min (bq b) (sq a)).
-         eapply matching_in_elim9 with (B:=(b::B))(A:=(a::A)).
-         all:auto. lia. split. destruct H10. destruct H8. lia.
-         apply H10. lia. lia.  apply H8.
-       }  
-       { assert(Haba:ttqa M0 a >=ttq_ab M0 b a).
-         eauto. 
-         eapply MM_exists_opt_k with (k:= S n)(A:=A)(a:=a)(B:=B)(b:=b) in H5.
-         destruct H5 as [OPT H5]. exists OPT. 
-         destruct H5. destruct H9.
-         split. apply H5. split. 
-         assert (Hmin:ttq_ab OPT b a <= Nat.min (bq b) (sq a)).
-         eapply matching_in_elim9 with (B:=(b::B))(A:=(a::A)).
-         apply H5. auto.
-         split. assert (Hmin:ttq_ab OPT b a <= Nat.min (bq b) (sq a)).
-         eapply matching_in_elim9 with (B:=(b::B))(A:=(a::A)).
-         all:auto. lia. split. destruct H10. destruct H8. lia.
-         apply H10. lia. lia.  apply H8.
-       }
-Qed. 
-
-
-Lemma matching_in_elim10 (B:list order)(A:list order)(M:list transaction)(a:order)(b:order)
-(NDA:NoDup (a::A))(NDB:NoDup (b::B)):
-Sorted by_dsp (a::A) ->
-Sorted by_dbp (b::B) ->
-b<a ->
-matching_in (b::B) (a::A) M ->
-~In a (asks_of M).
-Proof. intros. induction M as [|m M'].
-simpl. eauto.
-assert(ask_of m <= bid_of m).
-apply H2. auto.
-assert(In (ask_of m) (a::A)).
-apply H2. simpl. auto.
-assert(In (bid_of m) (b::B)).
-apply H2. simpl. auto.
-destruct H4;destruct H5.
-{
-subst. lia.
-}
-{
-eapply Sorted_elim2 with (x:=(bid_of m)) in H0.
-unfold by_dbp in H0. move /orP in H0.
-destruct H0. move /leP in H0. subst. lia.
-move /andP in H0. destruct H0. move /eqP in H0.
-subst. lia. apply by_dbp_refl. eauto.
-}
-{
-simpl.
-intro. destruct H6. subst. lia.
-assert(exists m', In m' M'/\a = ask_of m'). eauto.
-destruct H7 as [m0 H7]. destruct H7. 
-assert(ask_of m0 <= bid_of m0).
-apply H2. auto.
-eapply Sorted_elim2 with (x:=(bid_of m0)) in H0.
-unfold by_dbp in H0. move /orP in H0.
-destruct H0. move /leP in H0. subst. lia.
-move /andP in H0. destruct H0. move /eqP in H0.
-subst. lia. apply by_dbp_refl. apply H2.
-simpl. right. eauto.
-}
-{
-intro. simpl in H6. destruct H6.
-rewrite H6 in H4. assert(~In a A).
-eauto. eauto.
-assert(exists m', In m' M'/\a = ask_of m'). eauto.
-destruct H7 as [m0 H7]. destruct H7. 
-assert(ask_of m0 <= bid_of m0).
-apply H2. auto.
-eapply Sorted_elim2 with (x:=(bid_of m0)) in H0.
-unfold by_dbp in H0. move /orP in H0.
-destruct H0. move /leP in H0. subst. lia.
-move /andP in H0. destruct H0. move /eqP in H0.
-subst. lia. apply by_dbp_refl. apply H2.
-simpl. right. eauto.
-}
-Qed.
-
-
-Lemma matching_in_elim11 (B:list order)(A:list order)(M:list transaction)(a:order)(b:order)
-(NDA:NoDup (a::A))(NDB:NoDup (b::B)):
-Sorted by_dsp (a::A) ->
-Sorted by_dbp (b::B) ->
-b<a ->
-matching_in (b::B) (a::A) M ->
-matching_in (b::B) A M.
-Proof. intros. assert(~In a (asks_of M)).
-eapply matching_in_elim10 in H2. all:auto.
-split. split. apply H2.
-split. apply H2. apply H2.
-split. apply H2. assert(asks_of M [<=] a::A).
-apply H2. eauto. Qed.
-
-*)
-
-(*
-Theorem MM_aux_OPT (B:list order)(A:list order)(M:list transaction)
-(b:order)(a:order)(ta tb: nat)
-(NDA:NoDup (ida a::(idas_of A)))(NDB:NoDup (idb b::(idbs_of B)))
-(NZT: forall m : fill_type, In m M -> tq m > 0)
-(NZB: forall b0, In b0 ((Mk_bid (bp b) (btime b) (bq b - tb) (idb b))::B) -> (bq b0)>0)
-(NZA: forall a0, In a0 ((Mk_ask (sp a) (stime a) (sq a - ta) (ida a))::A) -> (sq a0)>0):
-Sorted by_dbp (b::B) -> 
-Sorted by_dsp (a::A) -> 
-matching_in ((Mk_bid (bp b) (btime b) (bq b - tb) (idb b))::B)
-                        ((Mk_ask (sp a) (stime a) (sq a - ta) (ida a))::A) M ->
-Is_IR M -> 
-QM(M) <= QM(MM_aux (b::B) (a::A) tb ta).
-Proof. intros. 
-assert(HBS: Sorted by_dbp ((Mk_bid (bp b) (btime b) (bq b - tb) (idb b))::B)).
-constructor. eauto. intros. 
-eapply Sorted_elim4 with (x0:=x) in H.
-destruct b;destruct x. auto. auto.
-assert(HAS: Sorted by_dsp ((Mk_ask (sp a) (stime a) (sq a - ta) (ida a))::A)).
-constructor. eauto. intros. 
-eapply Sorted_elim4 with (x0:=x) in H0.
-destruct a;destruct x. auto. auto.
-funelim (MM_aux (b::B) (a::A) tb ta).
-rewrite <- Heqcall. 
-destruct (Nat.leb a b) eqn: Hab.
-{ 
-  assert(Hab0: a <= b). move /leP in Hab. auto.
-  destruct (Nat.leb (QM(M)) (min (bq b - tb) (sq a - ta))) eqn:Hqab.
-  { 
-    move /leP in Hqab.
-    destruct (Nat.eqb (bq b - tb) (sq a - ta)). simpl. lia.
-    destruct (Nat.leb (bq b - tb) (sq a - ta)) eqn:Hle.
-    simpl. lia. simpl.
-    move /eqP in Hle. lia.
-  }
-  {
-    eapply MM_exists_opt in H5.
-    all:auto. 
-    destruct H5 as [M0 H5].
-    destruct H5. destruct H7. destruct H8. destruct H9. rewrite H9.
-    destruct (Nat.eqb (bq b - tb) (sq a - ta)) eqn: Hqabeq.
-    {
-      simpl. simpl in H8.
-      assert(HM0':exists M0', 
-      (matching_in l l0 M0')/\Is_IR M0'/\(QM(M0)=QM(M0') + (bq b - tb))/\
-      (forall m : fill_type, In m M0' -> tq m > 0)).
-      {
-        eapply exists_M0_reduced_bid_ask_matching in H5.
-        simpl in H5.
-        destruct H5 as [M1 H5]. exists M1. split. apply H5.
-        split. apply H5. split. apply H5. apply H5.
-        auto. simpl.
-        move /eqP in Hqabeq. lia.
-        auto.
-      }
-      destruct HM0' as [M0' HM0'].
-      replace (QM M0) with (QM M0' + (bq b - tb)).
-      cut(QM M0' <= QM (MM_aux l l0 0 0)). lia.
-      case l eqn: Hl. simp MM_aux.
-      simpl.
-      { simp UM_aux.
-        simpl.  
-        { destruct HM0'. 
-          apply matching_on_nilB in H11. 
-          rewrite H11.  simpl. lia. }
-      }
-      case l0 eqn: Hl0. simp MM_aux.
-        { simp UM_aux.
-          simpl. destruct HM0'. 
-          apply matching_on_nilA in H11. 
-          rewrite H11.  simpl. lia.
-        }
-      eapply H with (M:=M0'). all:auto.
-      eauto. eauto. apply HM0'. 
-      { intros.
-        destruct H11. subst b1. simpl. 
-        replace (bq b0 - 0) with (bq b0). eauto.
-        lia. eauto. 
-      }
-      { intros.
-            destruct H11. subst a1. simpl. 
-            replace (sq a0 - 0) with (sq a0). eauto.
-            lia. eauto. 
-      } 
-      eauto. 
-      eauto.
-      { replace (bq b0 - 0) with (bq b0).
-        replace (sq a0 - 0) with (sq a0).
-        destruct HM0'. destruct b0;destruct a0. intros. 
-        eapply H11.  lia. lia.
-      }  
-      apply HM0'.
-      { replace (bq b0 - 0) with (bq b0).
-            assert(Sorted by_dbp (b0 :: l1));eauto;destruct b0;auto.
-            lia.
-      }
-      { replace (sq a0 - 0) with (sq a0). 
-        assert(Sorted by_dsp (a0 :: l2));eauto;destruct a0;auto.
-        lia. 
-      }
-     destruct HM0'. destruct H12. destruct H13;auto.
-    }
-    {
-      destruct (Nat.leb (bq b - tb) (sq a - ta)) eqn:Hle.
-      {
-        simpl. simpl in H6.
-        case l eqn: Hl. simp MM_aux. simpl.
-        { simp UM_aux.
-          simpl. 
-          apply matching_on_bnill in H5.
-          simpl in H5. lia.
-        } 
-        assert(HM0':exists M0', (matching_in 
-        ((Mk_bid (bp b0) (btime b0) (bq b0 - 0) (idb b0))::l1) 
-        ((Mk_ask (sp a) (stime a) (sq a - (ta + (bq b - tb))) (ida a))::l0)
-         M0')
-        /\Is_IR M0'/\(QM(M0)=QM(M0') + (bq b - tb))/\
-          (forall m : fill_type, In m M0' -> tq m > 0)).
-        {
-         eapply exists_M0_reduced_ask_matching with (b:=
-         {|
-          bp := b;
-          btime := btime b;
-          bq := bq b - tb;
-          idb := idb b |}) in H5.
-         destruct H5 as [M1 H5]. exists M1.
-         all:auto. simpl in H5. 
-         replace (sq a - (ta + (bq b - tb))) with (sq a - ta - (bq b - tb)).
-         replace (bq b0 - 0) with (bq b0). 
-         replace ({| bp := b0; btime := btime b0; bq := bq b0; idb := idb b0 |})
-         with b0. split. eapply H5. split. apply H5.
-         split. apply H5. apply H5.
-         destruct b0. simpl. auto.
-         lia. lia. simpl in H8. simpl. auto.
-         move /leP in Hle. lia. 
-         move /eqP in Hqabeq. move /leP in Hle. 
-         simpl. lia.
-        } 
-        destruct HM0' as [M0' HM0'].
-        replace (QM M0) with (QM M0' + (bq b - tb)).
-        cut(QM M0' <= QM (MM_aux (b0 :: l1) (a :: l0) 0 (ta + (bq b - tb)))).
-        lia.
-        eapply H0 with (M:=M0'). all:auto.
-        eauto. all: try apply HM0'. 
-        { move /leP in Hle. intros.
-            destruct H11. subst b1. simpl.
-            replace (bq b0 - 0) with (bq b0). eauto.
-            lia. eauto.
-        }
-        { move /leP in Hle. intros.
-          destruct H11. subst a0. simpl. move /eqP in Hqabeq. lia. eauto. 
-        }
-        eauto.
-        { replace (bq b0 - 0) with (bq b0). destruct b0;auto. eauto. 
-            lia.
-        } 
-        {
-        constructor. eauto. intros. simpl.          
-        eapply Sorted_elim4 with (x0:=x) in H4.
-        destruct a;destruct x. unfold by_dsp. simpl.
-        unfold by_dsp in H4. simpl in H4. auto. auto.
-        }
-        destruct HM0'. destruct H12. destruct H13. lia. 
-      }
-      {
-        simpl. simpl in H6.
-        case l0 eqn: Hl0. simp MM_aux. simpl.
-        { simp UM_aux.
-          simpl. simpl in H5. 
-          apply matching_on_anill in H5.
-          simpl in H5. simpl. lia.
-        } 
-        assert(HM0':exists M0', (matching_in 
-       ((Mk_bid (bp b) (btime b) (bq b - (tb + (sq a - ta))) (idb b))::l)
-       ((Mk_ask (sp a0) (stime a0) (sq a0 - 0) (ida a0))::l1)
-       M0')
-       /\Is_IR M0'/\(QM(M0)=QM(M0') + (sq a - ta))/\
-       (forall m : fill_type, In m M0' -> tq m > 0)).
-        {
-         eapply exists_M0_reduced_bid_matching with (a:=
-         {|
-          sp := a;
-          stime := stime a;
-          sq := sq a - ta;
-          ida := ida a |}) in H5. all:auto.
-         destruct H5 as [M1 H5]. exists M1.
-         destruct H5. simpl in H5. 
-         replace (bq b - (tb + (sq a - ta))) with (bq b - tb - (sq a - ta)).
-         split. replace (sq a0 - 0) with (sq a0).
-         replace ({| sp := a0; stime := stime a0; sq := sq a0; ida := ida a0 |})
-         with a0. eapply H5. destruct a0. simpl. auto.
-         lia. simpl in H11. split. apply H11. split. apply H11.
-         apply H11. lia.
-         simpl.
-         move /leP in Hle. simpl in H8.  lia. 
-         move /eqP in Hqabeq. move /leP in Hle. 
-         simpl. lia.
-        }
-        destruct HM0' as [M0' HM0'].
-        replace (QM M0) with (QM M0' + (sq a - ta)).
-        cut(QM M0' <= QM (MM_aux (b :: l) (a0 :: l1) (tb + (sq a - ta)) 0)).
-        lia.
-        eapply H1 with (M:=M0'). all:auto.
-        eauto. all: try apply HM0'. 
-        { move /leP in Hle. intros.
-            destruct H11. subst b0. simpl.
-             move /eqP in Hqabeq. lia. eauto.
-        }
-        { move /leP in Hle. intros.
-          destruct H11. subst a1. simpl. 
-        replace (sq a0 - 0) with (sq a0). eauto. 
-        lia. eauto.
-        }
-        eauto.
-        { constructor. eauto. intros. simpl. 
-          eapply Sorted_elim4 with (x0:=x) in H3.
-          destruct b;destruct x. unfold by_dsp. simpl.
-          unfold by_dsp in H3. simpl in H3. auto. auto.
-        }
-        { replace (sq a0 - 0) with (sq a0). destruct a0;auto. eauto. 
-            lia.
-        } 
-        destruct HM0'. destruct H12. destruct H13. lia. 
-        }
-      }
-      simpl. move /leP in Hqab. lia. 
-    }
-  }
-  {
-  case l0 eqn: Hl0. 
-  assert(Hbla:b<a).
-  move /leP in Hab. lia.
-  apply matching_in_elim11 in H5.
-  apply matching_on_nilA in H5. 
-  rewrite H5. simpl. lia. eauto. eauto.
-  eauto. eauto. auto. apply H2. all:auto. eauto.
-  intros. destruct H7. subst a1. simpl. 
-  replace (sq a0 - 0) with (sq a0). eauto. lia. eauto.
-  eauto. apply matching_in_elim11 in H5. 
-  replace (sq a0 - 0) with (sq a0). 
-  destruct a0. apply H5. lia. eauto. eauto.
-  eauto. eauto. auto. simpl. move /leP in Hab. lia. 
-  replace (sq a0 - 0) with (sq a0). destruct a0;auto. eauto. 
-  lia.
-} 
-Qed. *)
+split. auto. split. auto. split. auto.  lia. Qed.
 
 
 Theorem MM_aux_optimal (B:list order)(A:list order)(M:list transaction):
@@ -586,11 +239,15 @@ destruct (PeanoNat.Nat.eqb (oprice a - oprice b) 0) eqn:price.
       { move /leP in Hqab. assert(Hv:Vol M >= Nat.min (oquantity b) (oquantity a)). lia.
         apply (MM_exists_opt B0 A0 _ _ _) in Hv. all:auto. destruct Hv as [OPT Hv]. 
         destruct Hv as [Hvu HvQ]. destruct HvQ as [HvQ Hv]. rewrite Hv.
-        match goal with |[ |- context[_ (Match (?x::B0) A0)]] => set(a1:=x) end.  
-        assert(HM0:exists M0, (Matching M0 (a1::B0) A0)/\
-        (Vol(OPT) = Vol(M0) + oquantity a)).  admit. destruct HM0 as [M0 HMv]. 
-        destruct HMv as [HMu HMQ]. rewrite HMQ. cut(Vol M0 <= Vol (Match (a1 :: B0) A0)).
-        lia. subst a1. apply H. all:simpl;auto. destruct H3 as [H3 H3a]. destruct H3a as [H3a H3b]. destruct H3b as [H3b H3c].
+        match goal with |[ |- context[_ (Match (?x::B0) A0)]] => set(b1:=x) end.  
+        assert(HM0:exists M0, (Matching M0 (b1::B0) A0)/\
+        (Vol(OPT) = Vol(M0) + oquantity a)). apply remove_ab_transactions_matching in Hvu. 
+        unfold reduced in Hvu. rewrite f1 in Hvu. simpl in Hvu. replace 
+        (Nat.min (oquantity b) (oquantity a)) with (oquantity a) in Hvu. 
+        subst b1. auto. lia. auto. auto. destruct HM0 as [M0 HMv]. 
+        destruct HMv as [HMu HMQ]. rewrite HMQ. cut(Vol M0 <= Vol (Match (b1 :: B0) A0)).
+        lia. subst b1. apply H. all:simpl;auto. destruct H3 as [H3 H3a]. destruct H3a as [H3a H3b]. 
+        destruct H3b as [H3b H3c].
         split.  simpl.  auto. split. eauto. split. simpl. auto. eauto. apply SortedreducedB with (b:=b).
         all:simpl;auto. apply Sorted_inv in H6. apply H6. 
         move /eqP in price. lia.
@@ -604,7 +261,10 @@ destruct (PeanoNat.Nat.eqb (oprice a - oprice b) 0) eqn:price.
         apply (MM_exists_opt B0 A0 _ _ _) in Hv. all:auto. destruct Hv as [OPT Hv]. 
         destruct Hv as [Hvu HvQ]. destruct HvQ as [HvQ Hv]. rewrite Hv.
         assert(HM0:exists M0, (Matching M0 B0 A0)/\
-        (Vol(OPT) = Vol(M0) + oquantity a)). admit. destruct HM0 as [M0 HMv]. 
+        (Vol(OPT) = Vol(M0) + oquantity a)). apply remove_ab_transactions_matching in Hvu. 
+        unfold reduced in Hvu. rewrite f1 in Hvu. simpl in Hvu. replace 
+        (Nat.min (oquantity b) (oquantity a)) with (oquantity a) in Hvu. 
+        auto. lia. auto. auto. destruct HM0 as [M0 HMv]. 
         destruct HMv as [HMu HMQ]. rewrite HMQ. cut(Vol M0 <= Vol (Match B0 A0)).
         lia. apply H0. all:simpl;auto. destruct H3 as [H3 H3a]. destruct H3a as [H3a H3b]. destruct H3b as [H3b H3c].
         split.  eauto. split. eauto. split. eauto. eauto. apply Sorted_inv in H5. apply H5.
@@ -622,27 +282,59 @@ destruct (PeanoNat.Nat.eqb (oprice a - oprice b) 0) eqn:price.
         destruct Hv as [Hvu HvQ]. destruct HvQ as [HvQ Hv]. rewrite Hv.
         match goal with |[ |- context[_ (Match B0 (?x::A0))]] => set(a1:=x) end.  
         assert(HM0:exists M0, (Matching M0 B0 (a1::A0))/\
-        (Vol(OPT) = Vol(M0) + oquantity b)). admit. destruct HM0 as [M0 HMv]. 
+        (Vol(OPT) = Vol(M0) + oquantity b)). apply remove_ab_transactions_matching in Hvu. 
+        unfold reduced in Hvu. rewrite f1 in Hvu. simpl in Hvu. replace 
+        (Nat.min (oquantity b) (oquantity a)) with (oquantity b) in Hvu. 
+        subst a1. auto. lia. auto. auto. destruct HM0 as [M0 HMv]. 
         destruct HMv as [HMu HMQ]. rewrite HMQ. cut(Vol M0 <= Vol (Match B0 (a1 :: A0))).
         lia. subst a1. apply H1. all:simpl;auto. destruct H3 as [H3 H3a]. destruct H3a as [H3a H3b]. 
         destruct H3b as [H3b H3c].  split. eauto. split. simpl. auto. split. eauto. simpl. auto.
         apply Sorted_inv in H5. apply H5.
-        (* apply SortedreducedA with (a:=a). all:simpl;auto. *) admit. 
-        move /eqP in price. lia.
+        apply SortedreducedA_rev with (a:=a). all:simpl;auto. move /eqP in price. lia.
       }
     }
   } apply H2. all:auto. eauto. apply Sorted_inv in H6. destruct H3 as [H3 H3a]. destruct H3a as [H3a H3b]. 
-    destruct H3b as [H3b H3c]. split.  simpl.  auto. split. eauto. split. simpl. auto. eauto.  admit. admit. 
-Admitted.
+    destruct H3b as [H3b H3c]. split.  simpl.  auto. split. eauto. split. simpl. auto. eauto.
+    apply Sorted_inv in H6. apply H6. clear H0 H H1 H2. split.
+    intro. intros. apply H7 in H. destruct H as [b0 H]. destruct H as [a0 H].
+    destruct H. destruct H0.  destruct H1.  destruct H2. destruct H8. 
+    simpl in H. destruct H. subst a0. simpl in H0. destruct H0. subst b0.
+    unfold tradable in H8. move /eqP in price. lia.  
+    unfold tradable in H8. move /eqP in price. 
+    apply Sorted_ointroB with (b:=b) in H. move /leP in H. lia. auto.
+    exists b0. exists a0. split. auto. split. auto. split. auto. split. auto. 
+    split. auto. split. apply H9. split. apply H9. split. apply H9. apply H9.
+    split. intros. apply H7. auto. intros. apply H7. auto. Qed.
 
 
 Lemma MM_optimal B A:
 admissible B A -> Is_max (MM B A) B A.
 Proof. unfold Is_max. intros. split. apply MM_Is_Matching. auto. unfold MM. 
-assert(Vol ((Match (Decr_Bid.sort B) (Decr_Ask.sort A))) = Vol (FOA (Match (Decr_Bid.sort B) (Decr_Ask.sort A)) A)).
-eapply FOA_correct. split. exact H. eapply Maching_permutation_full with (A1:=(Decr_Ask.sort A))(B1:=(Decr_Bid.sort B)).
-admit. admit. exact. apply Match_Matching. admit. admit. rewrite <- H1. apply MM_aux_optimal. 
-apply admissible_perm with (A1:=A)(B1:=B). admit. admit. auto. admit. admit. eapply Maching_permutation_full with (A1:=A)(B1:=B). admit. admit. exact. auto. Admitted.
-
+assert(Vol ((Match (Decr_Bid.sort B) (Decr_Ask.sort A))) = 
+Vol (FOA (Match (Decr_Bid.sort B) (Decr_Ask.sort A)) A)).
+eapply FOA_correct. split. exact H. 
+eapply Maching_permutation_full with (A1:=(Decr_Ask.sort A))(B1:=(Decr_Bid.sort B)).
+apply perm_sym. apply Permulation_perm.
+apply Decr_Bid.Permuted_sort.
+apply perm_sym. apply Permulation_perm.
+apply Decr_Ask.Permuted_sort.
+ exact. apply Match_Matching. 
+apply perm_nodup with (l:=(ids A)). apply ids_perm. apply Permulation_perm.
+apply Decr_Ask.Permuted_sort. apply H.
+apply perm_nodup with (l:=(ids B)). apply ids_perm. apply Permulation_perm.
+apply Decr_Bid.Permuted_sort. apply H.
+rewrite <- H1. apply MM_aux_optimal. 
+apply admissible_perm with (A1:=A)(B1:=B). 
+apply Permulation_perm.
+apply Decr_Bid.Permuted_sort.
+apply Permulation_perm.
+apply Decr_Ask.Permuted_sort.
+apply H. apply Decr_Bid.Sorted_sort. apply Decr_Ask.Sorted_sort.
+eapply Maching_permutation_full with (A1:=A)(B1:=B). 
+apply Permulation_perm.
+apply Decr_Bid.Permuted_sort.
+apply Permulation_perm.
+apply Decr_Ask.Permuted_sort.
+exact. auto. Qed.
 
 End MM.
